src/Spec/Example.v
@@ -650,169 +650,42 @@ Qed.
 
 (** Many-thread correctness *)
 
-Lemma compile_ok_atomic_exec_tid : forall T (p1 : proc _ _ T) p2,
-  @atomic_compile_ok _ _ opHi2T compile_op _ p1 p2 ->
-  forall tid s s' result evs,
-    exec_tid op_step tid s p1 s' result evs ->
-    exists result' evs',
-      exec_tid opHi_step tid s p2 s' result' evs' /\
-      traces_match (prepend tid evs TraceEmpty) (prepend tid evs' TraceEmpty) /\
-      match result with
-      | inl v => match result' with
-        | inl v' => v = v'
-        | inr _ => False
-        end
-      | inr p' => match result' with
-        | inl _ => False
-        | inr p'' => atomic_compile_ok compile_op p' p''
-        end
-      end.
+Theorem my_compile_correct :
+  compile_correct opHi2T compile_op op_step opHi_step.
 Proof.
-  induction 1; intros.
+  unfold compile_correct; intros.
+  destruct op.
 
-  - exec_tid_inv.
-    do 2 eexists; split.
+  + repeat atomic_exec_inv.
+    repeat step_inv.
+    simpl; intuition eauto 20.
+
+    replace (inc (inc s1 tid) tid) with (inc2 s1 tid).
+    replace (inc s1 tid tid + 1) with (s1 tid + 2).
+    econstructor.
+
+    unfold inc, state_upd.
+      destruct_ifs; omega.
+    unfold inc, inc2, state_upd; apply functional_extensionality; intros.
+      destruct_ifs; omega.
+
+  + repeat atomic_exec_inv.
+    repeat step_inv.
+    simpl; intuition eauto 20.
+
+    replace (dec (dec (dec s1 tid) tid) tid) with (dec3 s1 tid).
+    replace (dec (dec s1 tid) tid tid - 1) with (s1 tid - 3).
     constructor.
-    split.
-    simpl; eauto.
-    eauto.
 
-  - exec_tid_inv.
-    destruct op.
+    unfold dec, state_upd.
+      destruct_ifs; omega.
+    unfold dec, dec3, state_upd; apply functional_extensionality; intros.
+      destruct_ifs; omega.
 
-    + repeat atomic_exec_inv.
-      repeat step_inv.
-      do 2 eexists; split.
-      constructor.
-
-      replace (inc (inc s1 tid) tid) with (inc2 s1 tid).
-      constructor.
-
-      unfold inc, inc2, state_upd; apply functional_extensionality; intros.
-        destruct_ifs; omega.
-
-      split.
-      simpl; eauto.
-
-      unfold inc, inc2, state_upd;
-        destruct_ifs; omega.
-
-    + repeat atomic_exec_inv.
-      repeat step_inv.
-      do 2 eexists; split.
-      constructor.
-
-      replace (dec (dec (dec s1 tid) tid) tid) with (dec3 s1 tid).
-      constructor.
-
-      unfold dec, dec3, state_upd; apply functional_extensionality; intros.
-        destruct_ifs; omega.
-
-      split.
-      simpl; eauto 20.
-
-      unfold dec, dec3, state_upd;
-        destruct_ifs; omega.
-
-    + repeat atomic_exec_inv.
-      repeat step_inv.
-      do 2 eexists; split.
-      constructor.
-      constructor.
-
-      split.
-      simpl; eauto.
-      eauto.
-
-  - exec_tid_inv.
-    do 2 eexists; split.
-    constructor.
-    split.
-    simpl; eauto.
-    eauto.
-
-  - exec_tid_inv.
-    do 2 eexists; split.
-    constructor.
-    split.
-    simpl; eauto.
-    eauto.
-
-  - exec_tid_inv.
-    eapply IHatomic_compile_ok in H12.
-    repeat deex.
-
-    destruct result0; destruct result'; try solve [ exfalso; eauto ].
-
-    + do 2 eexists; split.
-      eauto.
-      split.
-      eauto.
-      subst; eauto.
-
-    + do 2 eexists; split.
-      eauto.
-      split.
-      eauto.
-      constructor.
-      eauto.
-      eauto.
-
-  - exec_tid_inv.
-    do 2 eexists; split.
-    constructor.
-    split.
-    simpl; eauto.
-    eauto.
-
-  - exec_tid_inv.
-    do 2 eexists; split.
-    constructor.
-    split.
-    simpl; eauto.
-    eauto.
+  + repeat atomic_exec_inv.
+    repeat step_inv.
+    simpl; intuition eauto 20.
 Qed.
-
-
-Theorem all_traces_match_0 :
-  forall ts1 (ts2 : @threads_state _ opHi2T),
-  proc_match (atomic_compile_ok compile_op) ts1 ts2 ->
-  traces_match_ts op_step opHi_step ts1 ts2.
-Proof.
-  unfold traces_match_ts; intros.
-  generalize dependent ts3.
-  induction H0; intros.
-  - eapply proc_match_pick with (tid := tid) in H2 as H'.
-    intuition try congruence.
-    repeat deex.
-    rewrite H3 in H; inversion H; clear H; subst.
-    repeat maybe_proc_inv.
-
-    edestruct compile_ok_atomic_exec_tid; eauto.
-    repeat deex.
-
-    edestruct IHexec.
-    shelve.
-    intuition idtac.
-
-    eexists; split.
-    eapply ExecOne with (tid := tid).
-      eauto.
-      eauto.
-      eauto.
-
-    eapply traces_match_prepend; eauto.
-    Unshelve.
-
-    destruct result, x; simpl in *; try solve [ exfalso; eauto ].
-    eapply proc_match_del; eauto.
-    eapply proc_match_upd; eauto.
-
-  - eexists; split.
-    eapply ExecEmpty; eauto.
-    eauto.
-Qed.
-
 
 Theorem my_atomize_correct :
   atomize_correct compile_op op_step.
@@ -837,63 +710,9 @@ Proof.
     eauto.
 Qed.
 
+Hint Resolve my_compile_correct.
 Hint Resolve my_atomize_correct.
 
-
-Theorem all_traces_match_1 :
-  forall ts1 ts1' (ts2 : @threads_state _ opHi2T),
-  proc_match (atomize_ok compile_op) ts1 ts1' ->
-  proc_match (atomic_compile_ok compile_op) ts1' ts2 ->
-  traces_match_ts op_step opHi_step ts1 ts2.
-Proof.
-  intros.
-  rewrite atomize_ok_hitrace_incl_ts; eauto.
-  eapply all_traces_match_0; eauto.
-Qed.
-
-Theorem make_one_atomic :
-  forall T (p2 : proc _ opHi2T T) (p1 : proc _ _ T),
-  compile_ok compile_op p1 p2 ->
-    atomize_ok compile_op p1 (compile (atomize compile_op) p2) /\
-    atomic_compile_ok compile_op (compile (atomize compile_op) p2) p2.
-Proof.
-  induction 1; simpl; intros.
-  - split. constructor. repeat constructor.
-  - split; constructor.
-  - intuition idtac.
-    constructor. eauto. intros. specialize (H1 x). intuition eauto.
-    constructor. eauto. intros. specialize (H1 x). intuition eauto.
-  - split; constructor.
-  - split; constructor.
-Qed.
-
-Hint Resolve proc_match_cons_Proc.
-Hint Resolve proc_match_cons_NoProc.
-
-
-Theorem make_all_atomic :
-  forall ts1 (ts2 : @threads_state _ opHi2T),
-  proc_match (compile_ok compile_op) ts1 ts2 ->
-  exists ts1',
-    proc_match (atomize_ok compile_op) ts1 ts1' /\
-    proc_match (atomic_compile_ok compile_op) ts1' ts2.
-Proof.
-  induction ts1; intros.
-  - eapply proc_match_len in H.
-    destruct ts3; simpl in *; try omega.
-    eexists; split.
-    eapply proc_match_nil.
-    eapply proc_match_nil.
-  - eapply proc_match_len in H as H'.
-    destruct ts3; simpl in *; try omega.
-
-    eapply proc_match_cons_inv in H.
-    edestruct IHts1; intuition eauto.
-    + exists (NoProc :: x); subst; intuition eauto.
-    + repeat deex.
-      edestruct (make_one_atomic H4).
-      eexists (Proc _ :: x); intuition eauto.
-Qed.
 
 Theorem all_traces_match :
   forall ts1 (ts2 : @threads_state _ opHi2T),
@@ -901,6 +720,5 @@ Theorem all_traces_match :
   traces_match_ts op_step opHi_step ts1 ts2.
 Proof.
   intros.
-  eapply make_all_atomic in H; deex.
-  eapply all_traces_match_1; eauto.
+  eapply compile_traces_match_ts; eauto.
 Qed.
